started dehn algorithm

DehnFunction/Dehn_algo_lemmas.lean
@@ -2,6 +2,8 @@ import DehnFunction.IsRed
 
 variable {α G : Type} [DecidableEq α] [Group G] [DecidableEq G]
 
+namespace FreeGroup
+
 /--
 For every g in l, this checks for cancellations in `a*g` or `a*g⁻¹`, and accordingly adds them when there are no such cancellations
 -/
@@ -15,13 +17,13 @@ def letter_mul_after_check_cancel (a : α) (l : List (FreeGroup α)) : List (Fre
     else [(.of a)*g,(.of a)⁻¹*g]++(letter_mul_after_check_cancel a gs)
 
 lemma IsRed.toWord (g : FreeGroup α) : IsRed g.toWord := by
-  rw [IsRed.iff_reduce_self]
+  rw [IsRed.equiv_of_reds]
   exact FreeGroup.reduce_toWord g
 
 lemma mul_toWord_noCancel1 (a : α) {g : FreeGroup α} (hg1 : g≠1) (hg2 : g.toWord.head (by contrapose! hg1; exact FreeGroup.toWord_eq_nil_iff.mp hg1) ≠ (a,false)) :
   ((.of a)*g).toWord = (a,true)::g.toWord := by
   simp [FreeGroup.toWord_mul,FreeGroup.toWord_of,List.cons_append,-FreeGroup.reduce.cons]
-  rw [← IsRed.iff_reduce_self,IsRed.cons_iff_not_red_pair]
+  rw [← IsRed.equiv_of_reds,IsRed.cons_iff_not_red_pair]
   constructor
   · exact IsRed.toWord g
   · simp at hg2
@@ -32,7 +34,7 @@ lemma mul_toWord_noCancel1 (a : α) {g : FreeGroup α} (hg1 : g≠1) (hg2 : g.to
 lemma mul_toWord_noCancel2 (a : α) {g : FreeGroup α} (hg1 : g≠1) (hg2 : g.toWord.head (by contrapose! hg1; exact FreeGroup.toWord_eq_nil_iff.mp hg1) ≠ (a,true)) :
   ((.of a)⁻¹*g).toWord = (a,false)::g.toWord := by
   simp [FreeGroup.toWord_mul,FreeGroup.invRev,FreeGroup.toWord_of,List.cons_append,-FreeGroup.reduce.cons]
-  rw [← IsRed.iff_reduce_self,IsRed.cons_iff_not_red_pair]
+  rw [← IsRed.equiv_of_reds,IsRed.cons_iff_not_red_pair]
   constructor
   · exact IsRed.toWord g
   · simp at hg2
@@ -85,7 +87,7 @@ List of all the elements of `FreeGroup α` of norm k.
 
 (A = alphabet written as a list)
 -/
-def FreeGroup.elts_norm_k (A : List α) (hA : A ≠ []) (k : ℕ) : List (FreeGroup α) :=
+def elts_norm_k (A : List α) (hA : A ≠ []) (k : ℕ) : List (FreeGroup α) :=
   match k with
   | 0 => [1]
   | p+1 => (List.map (fun a => letter_mul_after_check_cancel a (elts_norm_k A hA p)) A).flatten
@@ -95,15 +97,12 @@ List of all the elements of `FreeGroup α` of norm 0 to k.
 
 (A = alphabet written as a list)
 -/
-def FreeGroup.elts_upto_norm_k (A : List α) (hA : A ≠ []) (k : ℕ) : List (FreeGroup α) :=
+def elts_upto_norm_k (A : List α) (hA : A ≠ []) (k : ℕ) : List (FreeGroup α) :=
   match k with
   | 0 => [1]
   | p+1 => (elts_upto_norm_k A hA p)++(elts_norm_k A hA (p+1))
 
--- Should I define elts_norm_k and append from 1 to k?
---which defn better?
-
-theorem FreeGroup.elts_norm_k_correct1 (A : List α) (hA : A ≠ []) (k : ℕ) (g : FreeGroup α) (hg : g ∈ elts_norm_k A hA k) : g.norm = k := by
+theorem elts_norm_k_correct1 (A : List α) (hA : A ≠ []) (k : ℕ) (g : FreeGroup α) (hg : g ∈ elts_norm_k A hA k) : g.norm = k := by
   induction k generalizing g with
   | zero =>
     simp [elts_norm_k] at hg
@@ -118,7 +117,7 @@ theorem FreeGroup.elts_norm_k_correct1 (A : List α) (hA : A ≠ []) (k : ℕ) (
       · rcases hg with ⟨b,hbas,hgb⟩
         exact letter_mul_after_check_cancel_elt_norm b p ih g hgb
 
-lemma FreeGroup.norm_eq_one (g : FreeGroup α) (hg : g.norm = 1) : ∃ a : α, g.toWord = [(a,true)] ∨ g.toWord = [(a,false)] := by
+lemma norm_eq_one (g : FreeGroup α) (hg : g.norm = 1) : ∃ a : α, g.toWord = [(a,true)] ∨ g.toWord = [(a,false)] := by
   rw [norm] at hg
   generalize g.toWord = l at *
   match l with
@@ -126,7 +125,7 @@ lemma FreeGroup.norm_eq_one (g : FreeGroup α) (hg : g.norm = 1) : ∃ a : α, g
     use x.1
     aesop
 
-lemma FreeGroup.norm_succ (g : FreeGroup α) (n : ℕ) (hg : g.norm = n+1) :
+lemma norm_succ (g : FreeGroup α) (n : ℕ) (hg : g.norm = n+1) :
   ∃ (a : α) (h : FreeGroup α), h.norm = n ∧ (g.toWord = (a,true)::h.toWord ∨ g.toWord = (a,false)::h.toWord) := by
   rw [norm] at hg
   generalize hl : g.toWord = l at *
@@ -150,7 +149,7 @@ lemma FreeGroup.norm_succ (g : FreeGroup α) (n : ℕ) (hg : g.norm = n+1) :
       have h1 := IsRed.toWord g
       rw [hl] at h1
       have h2 := IsRed.tail _ h1
-      rw [IsRed.iff_reduce_self] at h2
+      rw [IsRed.equiv_of_reds] at h2
       specialize ih (mk xs) n
       rw [toWord_mk] at ih
       simp at hg
@@ -224,8 +223,8 @@ lemma letter_mul_after_check_cancel_mem' (a : α) (g h : FreeGroup α) (l : List
     · simp [letter_mul_after_check_cancel]
       split_ifs with h1 h2 h3 <;> simp [ih hh]
 
--- assume there exists a computable choice function
-theorem FreeGroup.elts_norm_k_correct2 (A : List α) (hA : ∀ a : α, a ∈ A) (hAe : A ≠ []) (k : ℕ) (g : FreeGroup α) (hg : g.norm = k) : g ∈ elts_norm_k A hAe k := by
+-- assume alphabet can be written as a list
+theorem elts_norm_k_correct2 (A : List α) (hA : ∀ a : α, a ∈ A) (hAe : A ≠ []) (k : ℕ) (g : FreeGroup α) (hg : g.norm = k) : g ∈ elts_norm_k A hAe k := by
   induction k generalizing g with
   | zero =>
     simp [elts_norm_k]
@@ -248,10 +247,10 @@ Proof that `elts_norm_k` contains exactly the elements of `FreeGroup α` of norm
 
 (A = alphabet written as a list, hA = proof of that)
 -/
-theorem FreeGroup.elts_norm_k_correct (A : List α) (hA : ∀ a : α, a ∈ A) (hAe : A ≠ []) (g : FreeGroup α) (k : ℕ) : g ∈ elts_norm_k A hAe k ↔ g.norm = k :=
+theorem elts_norm_k_correct (A : List α) (hA : ∀ a : α, a ∈ A) (hAe : A ≠ []) (g : FreeGroup α) (k : ℕ) : g ∈ elts_norm_k A hAe k ↔ g.norm = k :=
   ⟨fun h ↦ elts_norm_k_correct1 A hAe k g h,fun h ↦ elts_norm_k_correct2 A hA hAe k g h⟩
 
-theorem FreeGroup.elts_upto_norm_k_correct (A : List α) (hAe : A ≠ []) (k : ℕ) : elts_upto_norm_k A hAe k = (List.ofFn (fun (i:Fin (k+1)) => elts_norm_k A hAe i)).flatten := by
+theorem elts_upto_norm_k_correct (A : List α) (hAe : A ≠ []) (k : ℕ) : elts_upto_norm_k A hAe k = (List.ofFn (fun (i:Fin (k+1)) => elts_norm_k A hAe i)).flatten := by
   induction k with
   | zero =>
     simp [elts_upto_norm_k,elts_norm_k]
@@ -272,7 +271,7 @@ Proof that `elts_upto_norm_k` contains exactly the elements of `FreeGroup α` up
 
 (A = alphabet written as a list, hA = proof of that)
 -/
-theorem FreeGroup.set_of_words_norm_le_k_eq (A : List α) (hA : ∀ a : α, a ∈ A) (hAe : A ≠ []) (k : ℕ) : {g : FreeGroup α | FreeGroup.norm g ≤ k} = {x | x ∈ elts_upto_norm_k A hAe k} := by
+theorem set_of_words_norm_le_k_eq (A : List α) (hA : ∀ a : α, a ∈ A) (hAe : A ≠ []) (k : ℕ) : {g : FreeGroup α | FreeGroup.norm g ≤ k} = {x | x ∈ elts_upto_norm_k A hAe k} := by
   induction k with
   | zero =>
     simp [elts_upto_norm_k]
@@ -304,22 +303,175 @@ theorem FreeGroup.set_of_words_norm_le_k_eq (A : List α) (hA : ∀ a : α, a �
         exact Nat.le_of_eq hg
         exact hA
 
+theorem elts_upto_norm_k_correct' (A : List α) (hA : ∀ a : α, a ∈ A) (hAe : A ≠ []) (k : ℕ) (x : FreeGroup α) : x ∈ elts_upto_norm_k A hAe k ↔ x.norm ≤ k := by
+  change x ∈ {x | x ∈ elts_upto_norm_k A hAe k} ↔ x.norm ≤ k
+  rw [← set_of_words_norm_le_k_eq]
+  simp
+  exact hA
+
+end FreeGroup
+
 /--
-Given [r₁,...,rₙ] and [u₁,...,uₙ], it produces [u₁*r₁*u₁⁻¹,...,uₙ*rₙ*uₙ⁻¹]
+Given a list A, generates lists of size n out of the elements of A
 -/
-def lists_conjugate (rlist ulist : List G) : List G :=
-  match rlist,ulist with
-  | [],[] => []
-  | r::rs,[] => r::rs
-  | [],_::_ => []
-  | r::rs,u::us => u*r*u⁻¹::(lists_conjugate rs us)
+def lists_of_size_n (A : List α) (n : ℕ) : List (List α) :=
+  match n with
+  | 0 => [[]]
+  | k+1 => (List.map (fun a => (List.map (fun l => a::l)) (lists_of_size_n A k)) A).flatten
+
+-- #eval lists_of_size_n [1,2] 3
+
+#eval lists_of_size_n [1,2,3] 2
+omit [DecidableEq α] in
+/--
+The lists in `lists_of_size_n` are of size n
+-/
+lemma lists_of_size_n_size_eq_n (A : List α) (n : ℕ) : ∀ l ∈ lists_of_size_n A n, l.length = n := by
+  induction n with
+  | zero => simp [lists_of_size_n]
+  | succ k ih =>
+    intro l hl
+    simp [lists_of_size_n] at hl
+    rcases hl with ⟨a,ha,as,has1,has2⟩
+    specialize ih as has1
+    simpa [← has2]
+#check List.map
+
+omit [DecidableEq α] in
+/--
+The elements of the lists in `lists_of_size_n` lie in the original list
+-/
+lemma lists_of_size_n_elt_original (A : List α) (n : ℕ) (l : List α) (hl : l ∈ lists_of_size_n A n) : ∀ e ∈ l, e ∈ A := by
+  induction n generalizing l with
+  | zero => simp [lists_of_size_n] at hl; simp [hl]
+  | succ k ih =>
+    simp [lists_of_size_n] at hl
+    rcases hl with ⟨b,hb,bs,hb1,hb2⟩
+    specialize ih bs hb1
+    simp [← hb2]
+    exact ⟨hb,ih⟩
+
+omit [DecidableEq α] in
+/--
+If l is a list of size n containing only elements from A, it lies in `lists_of_size_n A n`
+-/
+lemma lists_of_size_n_elt_if (A : List α) (n : ℕ) (l : List α) (hl1 : l.length = n) (hl2 : ∀ e ∈ l, e ∈ A) : l ∈ lists_of_size_n A n := by
+  induction l generalizing n with
+  | nil =>
+    simp at hl1
+    simp [← hl1,lists_of_size_n]
+  | cons x xs ih =>
+    simp at hl1 hl2
+    simp [← hl1,lists_of_size_n]
+    specialize ih (n-1) (by rw [← hl1]; norm_num) hl2.2
+    constructor
+    · exact hl2.1
+    · convert ih
+      rw [← hl1]
+      norm_num
+
+-- /--
+-- Given [r₁,...,rₙ] and [u₁,...,uₙ], it produces [u₁*r₁*u₁⁻¹,...,u₁*rₙ*u₁⁻¹,...,uₙ*r₁*uₙ⁻¹,...,uₙ*rₙ*uₙ⁻¹]
+-- -/
+-- def lists_conjugate (rlist ulist : List G) : List G :=
+--   (List.map (fun r => (List.map (fun u => u*r*u⁻¹) ulist)) rlist).flatten
 
 inductive typ |a |b |c deriving DecidableEq, Repr
 
--- def alph := [typ.a,.b]
+def alph := [typ.a,.b]
 -- #eval (List.map FreeGroup.toWord (FreeGroup.elts_upto_norm_k ([typ.a,.b]) (by decide) 5))
 -- #eval (List.map FreeGroup.toWord (FreeGroup.elts_upto_norm_k ([typ.a,.b]) (by decide) 5)).length
 -- #eval (List.map FreeGroup.toWord (FreeGroup.elts_upto_norm_k ([typ.a,.b]) (by decide) 5)).Nodup
 
 -- def alph1 := [typ.a,.b,.c]
 -- #eval (List.map FreeGroup.toWord (FreeGroup.elts_upto_norm_k alph1 (by decide) 6)).length
+-- #eval List.map FreeGroup.toWord (lists_conjugate [(FreeGroup.of typ.a)*(.of .b)*(.of .a)⁻¹*(.of .b)⁻¹,(.of .b)] [(FreeGroup.of typ.a),(.of .a)⁻¹])
+
+/--
+Given [r₁,...,rₙ] and [u₁,...,uₙ], it produces [u₁*r₁*u₁⁻¹,u₂*r₂*u₂⁻¹,...,uₙ*rₙ*uₙ⁻¹]
+-/
+def produce_conjugated_term (rlist ulist : List G) : G :=
+  List.prod (aux rlist ulist) where
+  aux (rlist ulist : List G) :=
+    match rlist,ulist with
+    | l,[] => l
+    | [],_::_ => []
+    | r::rs,u::us => (u*r*u⁻¹)::(aux rs us)
+#eval (List.foldr max 5 [])
+
+namespace FreeGroup
+
+#check List.sublistsLen
+-- #eval List.sublistsLen 3 [1,2]
+def output_list_aux (rlist ulist : List (FreeGroup α)) (n : ℕ) : List (FreeGroup α) :=
+  let l1 := lists_of_size_n rlist n
+  let l2 := lists_of_size_n ulist n
+  (List.map (fun rs => (List.map (fun us => produce_conjugated_term rs us)) l2) l1).flatten
+
+/--Gives the maximum norm of all the elements in the list-/
+def list_max_norm (l : List (FreeGroup α)) : ℕ := List.foldr max 0 (List.map FreeGroup.norm l)
+
+/--The output list for the Dehn algorithm-/
+def output_list (rlist : List (FreeGroup α)) (dehn_bound : ℕ → ℕ) (n : ℕ) (A : List α) (hAe : A ≠ []) : List (FreeGroup α) :=
+  output_list_aux (rlist++(List.map (fun x => x⁻¹) rlist)) (elts_upto_norm_k A hAe (n + (list_max_norm rlist)*(dehn_bound n))) (dehn_bound n)
+
+def rels := [(FreeGroup.of typ.a)*(.of .b)]
+-- #eval list_max_norm [(FreeGroup.of typ.a)*(.of .b)]
+-- #eval FreeGroup.toWord ((lists_conjugate rels (elts_upto_norm_k alph (by decide) 3))).prod
+-- #eval List.map (fun l => List.map FreeGroup.toWord l) (lists_of_size_n rels 2)
+-- #eval (List.map FreeGroup.toWord (output_list [(FreeGroup.of typ.a)*(.of .b)] id 2 alph (by decide))).length
+
+-- rlist need not be relators here
+/--The output list of the Dehn algorithm is a list of the relators and their inverses conjugated by elements upto a certain norm-/
+lemma output_list_correct (rlist : List (FreeGroup α)) (dehn_bound : ℕ → ℕ) (n : ℕ) (A : List α) (hAe : A ≠ []) (hA : ∀ a : α, a ∈ A) (g : FreeGroup α) :
+  g ∈ output_list rlist dehn_bound n A hAe
+  ↔ ∃ rs us,
+  g = (produce_conjugated_term rs us)
+  ∧ rs.length = (dehn_bound n)
+  ∧ (∀ r ∈ rs, r ∈ rlist ++ (List.map (fun x => x⁻¹) rlist))
+  ∧ us.length = (dehn_bound n)
+  ∧ (∀ u ∈ us, u.norm ≤ (n + (list_max_norm rlist)*(dehn_bound n))) := by
+  constructor
+  · intro h
+    simp [output_list,output_list_aux] at h
+    rcases h with ⟨rs,hrs,us,hus,hg⟩
+    use rs
+    use us
+    simp [hg,lists_of_size_n_size_eq_n _ _ _ hrs,lists_of_size_n_size_eq_n _ _ _ hus,-List.mem_append]
+    constructor
+    · exact fun r a ↦ lists_of_size_n_elt_original _ (dehn_bound n) rs hrs r a
+    · apply lists_of_size_n_elt_original at hus
+      intro u hu
+      specialize hus u hu
+      rwa [elts_upto_norm_k_correct'] at hus
+      exact hA
+  · intro ⟨rs,us,hg,hrs1,hrs2,hus1,hus2⟩
+    simp [output_list,output_list_aux]
+    use rs
+    use lists_of_size_n_elt_if _ (dehn_bound n) rs hrs1 hrs2
+    use us
+    constructor
+    · apply lists_of_size_n_elt_if _ _ _ hus1
+      intro u hu
+      rw [elts_upto_norm_k_correct']
+      exact hus2 u hu
+      exact hA
+    · exact (Eq.symm hg)
+
+-- rlist needs to be list of relators here
+theorem word_in_reqd_list_aux (rlist : List (FreeGroup α)) (n : ℕ) (dehn_bound : ℕ → ℕ) (w : FreeGroup α) (hw : IsProductOfNConjugates {R | R ∈ rlist} (dehn_bound n) w) :
+  ∃ rs us,
+    w = (produce_conjugated_term rs us)
+    ∧ rs.length = (dehn_bound n)
+    ∧ (∀ r ∈ rs, r ∈ (rlist) ++ (List.map (fun x => x⁻¹) rlist))
+    ∧ us.length = (dehn_bound n)
+    ∧ (∀ u ∈ us, u.norm ≤ (n + (list_max_norm rlist)*(dehn_bound n))) := by sorry
+
+-- w is identity in place of prod n conj
+theorem word_in_reqd_list (rlist : List (FreeGroup α)) (n : ℕ) (dehn_bound : ℕ → ℕ) (w : FreeGroup α) (hw : IsProductOfNConjugates {R | R ∈ rlist} (dehn_bound n) w) (A : List α) (hAe : A ≠ []) (hA : ∀ a : α, a ∈ A) :
+  w ∈ output_list rlist dehn_bound n A hAe :=
+  (output_list_correct rlist dehn_bound n A hAe hA w).mpr (word_in_reqd_list_aux rlist n dehn_bound w hw)
+
+--if w=1 it is in output list (decidable dehn bound)
+
+end FreeGroup
